Revise the Stacking pass and its proof to make it easier to adapt to 64-bit architectures
The original Stacking pass and its proof hard-wire assumptions about the processor and the register allocation, namely that integer registers are 32 bit wide and that all stack slots have natural alignment 4, which precludes having stack slots of type Tlong.  Those assumptions become false if the target processor has 64-bit integer registers.

This commit makes minimal adjustments to the Stacking pass so as to lift these assumptions:
- Stack slots of type Tlong (or more generally of natural alignment 8) are supported.  For slots produced by register allocation, the alignment is validated a posteriori in Lineartyping.  For slots produced by the calling conventions, alignment is proved as part of the "loc_argument_acceptable" property in Conventions1.
- The code generated by Stacking to save and restore used callee-save registers no longer assumes 32-bit integer registers.  Actually, it supports any combination of sizes for registers.
- To support the new save/restore code, Bounds was changed to record the set of all callee-save registers used, rather than just the max index of callee-save registers used.

On CompCert's current 32-bit target architectures, the new Stacking pass should generate pretty much the same code as the old one, modulo minor differences in the layout of the stack frame.  (E.g. padding could be introduced at different places.)

The bulk of this big commit is related to the proof of the Stacking phase.  The old proof strategy was painful and not obviously adaptable to the new Stacking phase, so I rewrote Stackingproof entirely, using an approach inspired by separation logic.  The new library common/Separation.v defines assertions about memory states that can be composed using a separating conjunction, just like pre- and post-conditions in separation logic.  Those assertions are used in Stackingproof to describe the contents of the stack frames during the execution of the generated Mach code, and relate them with the Linear location maps.

As a further simplification, the callee-save/caller-save distinction is now defined in Conventions1 by a function is_callee_save: mreg -> bool, instead of lists of registers of either kind as before.  This eliminates many boring classification lemmas from Conventions1.  LTL and Lineartyping were adapted accordingly.

Finally, this commit introduces a new library called Decidableplus to prove some propositions by reflection as Boolean computations.  It is used to further simplify the proofs in Conventions1.

backend/IRC.ml
@@ -833,10 +833,10 @@ let find_slot conflicts typ =
   | [] ->
       S(Local, curr, typ)
   | S(Local, ofs, typ') :: l ->
-      if Z.le (Z.add curr (typesize typ)) ofs then
+      if Z.le (Z.add curr (Locations.typesize typ)) ofs then
         S(Local, curr, typ)
       else begin
-        let ofs' = Z.add ofs (typesize typ') in
+        let ofs' = Z.add ofs (Locations.typesize typ') in
         find (if Z.le ofs' curr then curr else ofs') l
       end
   | _ :: l ->
