ia32/Machregsaux.ml
@@ -30,7 +30,4 @@ let name_of_register r =
 let register_by_name s =
   Machregs.register_by_name (coqstring_of_camlstring (String.uppercase s))
 
-let can_reserve_register r =
-  List.mem r Conventions1.int_callee_save_regs
-  || List.mem r Conventions1.float_callee_save_regs
-
+let can_reserve_register r = Conventions1.is_callee_save r
