arm/Conventions1.v
@@ -14,6 +14,7 @@
     machine registers and stack slots. *)
 
 Require Import Coqlib.
+Require Import Decidableplus.
 Require Import AST.
 Require Import Events.
 Require Import Locations.
@@ -33,6 +34,14 @@ Require Archi.
   of callee- and caller-save registers.
 *)
 
+Definition is_callee_save (r: mreg): bool :=
+  match r with
+  | R0  | R1  | R2  | R3  | R12 => false
+  | R4  | R5  | R6  | R7  | R8  | R9  | R10 | R11 => true
+  | F0  | F1  | F2  | F3  | F4  | F5  | F6  | F7 => false
+  | F8  | F9  | F10  | F11 | F12  | F13  | F14  | F15 => true
+  end.
+
 Definition int_caller_save_regs :=
   R0 :: R1 :: R2 :: R3 :: R12 :: nil.
 
@@ -46,170 +55,10 @@ Definition float_callee_save_regs :=
   F8 :: F9 :: F10 :: F11 :: F12 :: F13 :: F14 :: F15 :: nil.
 
 Definition destroyed_at_call :=
-  int_caller_save_regs ++ float_caller_save_regs.
+  List.filter (fun r => negb (is_callee_save r)) all_mregs.
 
 Definition dummy_int_reg := R0.     (**r Used in [Coloring]. *)
 Definition dummy_float_reg := F0.   (**r Used in [Coloring]. *)
-
-(** The [index_int_callee_save] and [index_float_callee_save] associate
-  a unique positive integer to callee-save registers.  This integer is
-  used in [Stacking] to determine where to save these registers in
-  the activation record if they are used by the current function. *)
-
-Definition index_int_callee_save (r: mreg) :=
-  match r with
-  | R4 => 0  | R5 => 1  | R6 => 2  | R7 => 3
-  | R8 => 4  | R9 => 5  | R10 => 6 | R11 => 7
-  | _ => -1
-  end.
-
-Definition index_float_callee_save (r: mreg) :=
-  match r with
-  | F8 => 0  | F9 => 1  | F10 => 2  | F11 => 3
-  | F12 => 4  | F13 => 5  | F14 => 6  | F15 => 7
-  | _ => -1
-  end.
-
-Ltac ElimOrEq :=
-  match goal with
-  |  |- (?x = ?y) \/ _ -> _ =>
-       let H := fresh in
-       (intro H; elim H; clear H;
-        [intro H; rewrite <- H; clear H | ElimOrEq])
-  |  |- False -> _ =>
-       let H := fresh in (intro H; contradiction)
-  end.
-
-Ltac OrEq :=
-  match goal with
-  | |- (?x = ?x) \/ _ => left; reflexivity
-  | |- (?x = ?y) \/ _ => right; OrEq
-  | |- False => fail
-  end.
-
-Ltac NotOrEq :=
-  match goal with
-  | |- (?x = ?y) \/ _ -> False =>
-       let H := fresh in (
-       intro H; elim H; clear H; [intro; discriminate | NotOrEq])
-  | |- False -> False =>
-       contradiction
-  end.
-
-Lemma index_int_callee_save_pos:
-  forall r, In r int_callee_save_regs -> index_int_callee_save r >= 0.
-Proof.
-  intro r. simpl; ElimOrEq; unfold index_int_callee_save; omega.
-Qed.
-
-Lemma index_float_callee_save_pos:
-  forall r, In r float_callee_save_regs -> index_float_callee_save r >= 0.
-Proof.
-  intro r. simpl; ElimOrEq; unfold index_float_callee_save; omega.
-Qed.
-
-Lemma index_int_callee_save_pos2:
-  forall r, index_int_callee_save r >= 0 -> In r int_callee_save_regs.
-Proof.
-  destruct r; simpl; intro; omegaContradiction || OrEq.
-Qed.
-
-Lemma index_float_callee_save_pos2:
-  forall r, index_float_callee_save r >= 0 -> In r float_callee_save_regs.
-Proof.
-  destruct r; simpl; intro; omegaContradiction || OrEq.
-Qed.
-
-Lemma index_int_callee_save_inj:
-  forall r1 r2,
-  In r1 int_callee_save_regs ->
-  In r2 int_callee_save_regs ->
-  r1 <> r2 ->
-  index_int_callee_save r1 <> index_int_callee_save r2.
-Proof.
-  intros r1 r2.
-  simpl; ElimOrEq; ElimOrEq; unfold index_int_callee_save;
-  intros; congruence.
-Qed.
-
-Lemma index_float_callee_save_inj:
-  forall r1 r2,
-  In r1 float_callee_save_regs ->
-  In r2 float_callee_save_regs ->
-  r1 <> r2 ->
-  index_float_callee_save r1 <> index_float_callee_save r2.
-Proof.
-  intros r1 r2.
-  simpl; ElimOrEq; ElimOrEq; unfold index_float_callee_save;
-  intros; congruence.
-Qed.
-
-(** The following lemmas show that
-    (temporaries, destroyed at call, integer callee-save, float callee-save)
-    is a partition of the set of machine registers. *)
-
-Lemma int_float_callee_save_disjoint:
-  list_disjoint int_callee_save_regs float_callee_save_regs.
-Proof.
-  red; intros r1 r2. simpl; ElimOrEq; ElimOrEq; discriminate.
-Qed.
-
-Lemma register_classification:
-  forall r,
-  In r destroyed_at_call \/ In r int_callee_save_regs \/ In r float_callee_save_regs.
-Proof.
-  destruct r;
-  try (left; simpl; OrEq);
-  try (right; left; simpl; OrEq);
-  try (right; right; simpl; OrEq).
-Qed.
-
-
-Lemma int_callee_save_not_destroyed:
-  forall r,
-    In r destroyed_at_call -> In r int_callee_save_regs -> False.
-Proof.
-  intros. revert H0 H. simpl. ElimOrEq; NotOrEq.
-Qed.
-
-Lemma float_callee_save_not_destroyed:
-  forall r,
-    In r destroyed_at_call -> In r float_callee_save_regs -> False.
-Proof.
-  intros. revert H0 H. simpl. ElimOrEq; NotOrEq.
-Qed.
-
-Lemma int_callee_save_type:
-  forall r, In r int_callee_save_regs -> mreg_type r = Tany32.
-Proof.
-  intro. simpl; ElimOrEq; reflexivity.
-Qed.
-
-Lemma float_callee_save_type:
-  forall r, In r float_callee_save_regs -> mreg_type r = Tany64.
-Proof.
-  intro. simpl; ElimOrEq; reflexivity.
-Qed.
-
-Ltac NoRepet :=
-  match goal with
-  | |- list_norepet nil =>
-      apply list_norepet_nil
-  | |- list_norepet (?a :: ?b) =>
-      apply list_norepet_cons; [simpl; intuition discriminate | NoRepet]
-  end.
-
-Lemma int_callee_save_norepet:
-  list_norepet int_callee_save_regs.
-Proof.
-  unfold int_callee_save_regs; NoRepet.
-Qed.
-
-Lemma float_callee_save_norepet:
-  list_norepet float_callee_save_regs.
-Proof.
-  unfold float_callee_save_regs; NoRepet.
-Qed.
 
 (** * Function calling conventions *)
 
@@ -260,12 +109,12 @@ Qed.
 
 Lemma loc_result_caller_save:
   forall (s: signature) (r: mreg),
-  In r (loc_result s) -> In r destroyed_at_call.
+  In r (loc_result s) -> is_callee_save r = false.
 Proof.
   intros.
   assert (r = R0 \/ r = R1 \/ r = F0).
     unfold loc_result in H. destruct (sig_res s); [destruct t|idtac]; simpl in H; intuition.
-  destruct H0 as [A | [A | A]]; subst r; simpl; OrEq.
+  destruct H0 as [A | [A | A]]; subst r; auto.
 Qed.
 
 (** ** Location of function arguments *)
@@ -425,8 +274,8 @@ Definition size_arguments (s: signature) : Z :=
 
 Definition loc_argument_acceptable (l: loc) : Prop :=
   match l with
-  | R r => In r destroyed_at_call
-  | S Outgoing ofs ty => ofs >= 0 /\ ty <> Tlong
+  | R r => is_callee_save r = false
+  | S Outgoing ofs ty => ofs >= 0 /\ (typealign ty | ofs)
   | _ => False
   end.
 
@@ -451,20 +300,20 @@ Remark loc_arguments_hf_charact:
   In l (loc_arguments_hf tyl ir fr ofs) ->
   match l with
   | R r => In r int_param_regs \/ In r float_param_regs
-  | S Outgoing ofs' ty => ofs' >= ofs /\ ty <> Tlong
+  | S Outgoing ofs' ty => ofs' >= ofs /\ typealign ty = 1
   | S _ _ _ => False
   end.
 Proof.
   assert (INCR: forall l ofs1 ofs2,
             match l with
             | R r => In r int_param_regs \/ In r float_param_regs
-            | S Outgoing ofs' ty => ofs' >= ofs2 /\ ty <> Tlong
+            | S Outgoing ofs' ty => ofs' >= ofs2 /\ typealign ty = 1
             | S _ _ _ => False
             end ->
             ofs1 <= ofs2 ->
             match l with
             | R r => In r int_param_regs \/ In r float_param_regs
-            | S Outgoing ofs' ty => ofs' >= ofs1 /\ ty <> Tlong
+            | S Outgoing ofs' ty => ofs' >= ofs1 /\ typealign ty = 1
             | S _ _ _ => False
             end).
   {
@@ -477,13 +326,13 @@ Proof.
   destruct (zlt ir 4); destruct H.
   subst. left; apply ireg_param_in_params.
   eapply IHtyl; eauto.
-  subst. split; [omega | congruence].
+  subst. split; [omega | auto].
   eapply INCR. eapply IHtyl; eauto. omega.
 - (* float *)
   destruct (zlt fr 8); destruct H.
   subst. right; apply freg_param_in_params.
   eapply IHtyl; eauto.
-  subst. split. apply Zle_ge. apply align_le. omega. congruence.
+  subst. split. apply Zle_ge. apply align_le. omega. auto.
   eapply INCR. eapply IHtyl; eauto.
   apply Zle_trans with (align ofs 2). apply align_le; omega. omega.
 - (* long *)
@@ -493,26 +342,26 @@ Proof.
   destruct H. subst l; left; apply ireg_param_in_params.
   destruct H. subst l; left; apply ireg_param_in_params.
   eapply IHtyl; eauto.
-  destruct H. subst l; split; [ omega | congruence ].
-  destruct H. subst l; split; [ omega | congruence ].
+  destruct H. subst l; split; [ omega | auto ].
+  destruct H. subst l; split; [ omega | auto ].
   eapply INCR. eapply IHtyl; eauto. omega.
 - (* single *)
   destruct (zlt fr 8); destruct H.
   subst. right; apply freg_param_in_params.
   eapply IHtyl; eauto.
-  subst. split; [omega | congruence].
+  subst. split; [omega | auto].
   eapply INCR. eapply IHtyl; eauto. omega.
 - (* any32 *)
   destruct (zlt ir 4); destruct H.
   subst. left; apply ireg_param_in_params.
   eapply IHtyl; eauto.
-  subst. split; [omega | congruence].
+  subst. split; [omega | auto].
   eapply INCR. eapply IHtyl; eauto. omega.
 - (* any64 *)
   destruct (zlt fr 8); destruct H.
   subst. right; apply freg_param_in_params.
   eapply IHtyl; eauto.
-  subst. split. apply Zle_ge. apply align_le. omega. congruence.
+  subst. split. apply Zle_ge. apply align_le. omega. auto.
   eapply INCR. eapply IHtyl; eauto.
   apply Zle_trans with (align ofs 2). apply align_le; omega. omega.
 Qed.
@@ -522,20 +371,20 @@ Remark loc_arguments_sf_charact:
   In l (loc_arguments_sf tyl ofs) ->
   match l with
   | R r => In r int_param_regs \/ In r float_param_regs
-  | S Outgoing ofs' ty => ofs' >= Zmax 0 ofs /\ ty <> Tlong
+  | S Outgoing ofs' ty => ofs' >= Zmax 0 ofs /\ typealign ty = 1
   | S _ _ _ => False
   end.
 Proof.
   assert (INCR: forall l ofs1 ofs2,
             match l with
             | R r => In r int_param_regs \/ In r float_param_regs
-            | S Outgoing ofs' ty => ofs' >= Zmax 0 ofs2 /\ ty <> Tlong
+            | S Outgoing ofs' ty => ofs' >= Zmax 0 ofs2 /\ typealign ty = 1
             | S _ _ _ => False
             end ->
             ofs1 <= ofs2 ->
             match l with
             | R r => In r int_param_regs \/ In r float_param_regs
-            | S Outgoing ofs' ty => ofs' >= Zmax 0 ofs1 /\ ty <> Tlong
+            | S Outgoing ofs' ty => ofs' >= Zmax 0 ofs1 /\ typealign ty = 1
             | S _ _ _ => False
             end).
   {
@@ -548,7 +397,7 @@ Proof.
   destruct H.
   destruct (zlt ofs 0); subst l.
   left; apply ireg_param_in_params.
-  split. xomega. congruence.
+  split. xomega. auto.
   eapply INCR. eapply IHtyl; eauto. omega.
 - (* float *)
   set (ofs' := align ofs 2) in *.
@@ -556,7 +405,7 @@ Proof.
   destruct H.
   destruct (zlt ofs' 0); subst l.
   right; apply freg_param_in_params.
-  split. xomega. congruence.
+  split. xomega. auto.
   eapply INCR. eapply IHtyl; eauto. omega.
 - (* long *)
   set (ofs' := align ofs 2) in *.
@@ -564,23 +413,23 @@ Proof.
   destruct H.
   destruct (zlt ofs' 0); subst l.
   left; apply ireg_param_in_params.
-  split. xomega. congruence.
+  split. xomega. auto.
   destruct H.
   destruct (zlt ofs' 0); subst l.
   left; apply ireg_param_in_params.
-  split. xomega. congruence.
+  split. xomega. auto.
   eapply INCR. eapply IHtyl; eauto. omega.
 - (* single *)
   destruct H.
   destruct (zlt ofs 0); subst l.
   right; apply freg_param_in_params.
-  split. xomega. congruence.
+  split. xomega. auto.
   eapply INCR. eapply IHtyl; eauto. omega.
 - (* any32 *)
   destruct H.
   destruct (zlt ofs 0); subst l.
   left; apply ireg_param_in_params.
-  split. xomega. congruence.
+  split. xomega. auto.
   eapply INCR. eapply IHtyl; eauto. omega.
 - (* any64 *)
   set (ofs' := align ofs 2) in *.
@@ -588,7 +437,7 @@ Proof.
   destruct H.
   destruct (zlt ofs' 0); subst l.
   right; apply freg_param_in_params.
-  split. xomega. congruence.
+  split. xomega. auto.
   eapply INCR. eapply IHtyl; eauto. omega.
 Qed.
 
@@ -597,14 +446,18 @@ Lemma loc_arguments_acceptable:
   In l (loc_arguments s) -> loc_argument_acceptable l.
 Proof.
   unfold loc_arguments; intros.
-  assert (forall r, In r int_param_regs \/ In r float_param_regs -> In r destroyed_at_call).
-  {
-    intros. elim H0; simpl; ElimOrEq; OrEq.
-  }
+  assert (A: forall r, In r int_param_regs -> is_callee_save r = false) by decide_goal.
+  assert (B: forall r, In r float_param_regs -> is_callee_save r = false) by decide_goal.
+  assert (C: forall r, In r int_param_regs \/ In r float_param_regs -> is_callee_save r = false).
+  { intros. destruct H0; auto. }
   assert (In l (loc_arguments_sf (sig_args s) (-4)) -> loc_argument_acceptable l).
-  { intros. red. exploit loc_arguments_sf_charact; eauto. destruct l; auto. }
+  { intros. red. exploit loc_arguments_sf_charact; eauto.
+    destruct l as [r | [] ofs ty]; auto. 
+    intros [P Q]. rewrite Q; split. auto. apply Z.divide_1_l. }
   assert (In l (loc_arguments_hf (sig_args s) 0 0 0) -> loc_argument_acceptable l).
-  { intros. red. exploit loc_arguments_hf_charact; eauto. destruct l; auto. }
+  { intros. red. exploit loc_arguments_hf_charact; eauto.
+    destruct l as [r | [] ofs ty]; auto. 
+    intros [P Q]. rewrite Q; split. auto. apply Z.divide_1_l. }
   destruct Archi.abi; [ | destruct (cc_vararg (sig_cc s)) ]; auto.
 Qed.
 
