arm/Machregs.v
@@ -12,6 +12,7 @@
 
 Require Import String.
 Require Import Coqlib.
+Require Import Decidableplus.
 Require Import Maps.
 Require Import AST.
 Require Import Op.
@@ -43,6 +44,26 @@ Lemma mreg_eq: forall (r1 r2: mreg), {r1 = r2} + {r1 <> r2}.
 Proof. decide equality. Defined.
 Global Opaque mreg_eq.
 
+Definition all_mregs :=
+     R0  :: R1  :: R2  :: R3 :: R4  :: R5  :: R6  :: R7
+  :: R8  :: R9  :: R10 :: R11 :: R12
+  :: F0  :: F1  :: F2  :: F3  :: F4  :: F5  :: F6  :: F7
+  :: F8  :: F9  :: F10 :: F11 :: F12 :: F13 :: F14 :: F15 :: nil.
+
+Lemma all_mregs_complete:
+  forall (r: mreg), In r all_mregs.
+Proof.
+  assert (forall r, proj_sumbool (In_dec mreg_eq r all_mregs) = true) by (destruct r; reflexivity).
+  intros. specialize (H r). InvBooleans. auto.
+Qed.
+
+Instance Decidable_eq_mreg : forall (x y: mreg), Decidable (eq x y) := Decidable_eq mreg_eq.
+  
+Instance Finite_mreg : Finite mreg := {
+  Finite_elements := all_mregs;
+  Finite_elements_spec := all_mregs_complete
+}.
+
 Definition mreg_type (r: mreg): typ :=
   match r with
   | R0  | R1  | R2  | R3   | R4  | R5  | R6  | R7
@@ -70,7 +91,7 @@ Module IndexedMreg <: INDEXED_TYPE.
   Lemma index_inj:
     forall r1 r2, index r1 = index r2 -> r1 = r2.
   Proof.
-    destruct r1; destruct r2; simpl; intro; discriminate || reflexivity.
+    decide_goal.
   Qed.
 End IndexedMreg.
 
