backend/Locations.v
@@ -84,6 +84,28 @@ Proof.
   destruct ty; compute; auto.
 Qed.
 
+Definition typealign (ty: typ) : Z :=
+  match ty with
+  | Tint => 1
+  | Tlong => 2
+  | Tfloat => 1
+  | Tsingle => 1
+  | Tany32 => 1
+  | Tany64 => 1
+  end.
+
+Lemma typealign_pos:
+  forall (ty: typ), typealign ty > 0.
+Proof.
+  destruct ty; compute; auto.
+Qed.
+
+Lemma typealign_typesize:
+  forall (ty: typ), (typealign ty | typesize ty).
+Proof.
+  intros. exists (typesize ty / typealign ty); destruct ty; reflexivity.
+Qed.
+
 (** ** Locations *)
 
 (** Locations are just the disjoint union of machine registers and
