extraction/extraction.v
@@ -159,6 +159,8 @@ Separate Extraction
    Ctyping.typecheck_program
    Ctyping.epostincr Ctyping.epostdecr Ctyping.epreincr Ctyping.epredecr
    Ctypes.make_program
+   Conventions1.int_caller_save_regs Conventions1.float_caller_save_regs 
+   Conventions1.int_callee_save_regs Conventions1.float_callee_save_regs 
    Conventions1.dummy_int_reg Conventions1.dummy_float_reg
    RTL.instr_defs RTL.instr_uses
    Machregs.mregs_for_operation Machregs.mregs_for_builtin
